test/UnicodeAlphabetic.ml
@@ -1,0 +1,31 @@
+open! Warblre.Extracted.Patterns
+open Warblre.Helpers
+open Warblre.Notations
+
+let%expect_test "ascii" =
+  test_regex
+    (!* (uprop "Alphabetic"))
+    "abcdefghijklmnopqrstuvwxyzABCDEFGHIJKLMNOPQRSTUVWXYZ"
+    0 ();
+  [%expect {| Matched 52 characters ([0-52]) in 'abcdefghijklmnopqrstuvwxyzABCDEFGHIJKLMNOPQRSTUVWXYZ' (length=52) |}]
+
+let%expect_test "space" =
+  test_regex
+    (!* (uprop "Alphabetic"))
+    "abcdefghijklmno pqrstuvwxyzABCDEFGHIJKLMNOPQRSTUVWXYZ"
+    0 ();
+  [%expect {| Matched 15 characters ([0-15]) in 'abcdefghijklmno pqrstuvwxyzABCDEFGHIJKLMNOPQRSTUVWXYZ' (length=53) |}]
+
+let%expect_test "tab" =
+  test_regex
+    (!* (uprop "Alphabetic"))
+    "abcdefghijklmno\tpqrstuvwxyzABCDEFGHIJKLMNOPQRSTUVWXYZ"
+    0 ();
+  [%expect {| Matched 15 characters ([0-15]) in 'abcdefghijklmno	pqrstuvwxyzABCDEFGHIJKLMNOPQRSTUVWXYZ' (length=53) |}]
+
+let%expect_test "greek" =
+  test_regex
+    (!* (uprop "Alphabetic"))
+    "αβγδεϝͷϛζͱηθιϳκλμνξοπϻϟϙρσͼτυφχψωϡͳϸ"
+    0 ();
+  [%expect {| Matched 36 characters ([0-36]) in 'αβγδεϝͷϛζͱηθιϳκλμνξοπϻϟϙρσͼτυφχψωϡͳϸ' (length=36) |}]
