MECMAR/utils/Typeclasses.v
@@ -1,5 +1,5 @@
 Module EqDec.
-  Class type (T: Type) := {
+  Class type (T: Type) := make {
     eq_dec: forall (l r: T), {l=r} + {l<>r};
   }.
 
@@ -17,5 +17,6 @@ Infix "!=" := EqDec.neqb (at level 37, no associativity).
 From Coq Require Import ZArith.
 Instance eqdec_bool: EqDec bool := { eq_dec := Bool.bool_dec }.
 Instance eqdec_nat: EqDec nat := { eq_dec := Nat.eq_dec }.
+Instance eqdec_string: EqDec String.string := { eq_dec := String.string_dec }.
 #[refine] Instance eqdec_positive: EqDec positive := {}. decide equality. Defined.
 #[refine] Instance eqdec_option {T: Type} `{EqDec T}: EqDec (option T) := {}. decide equality; apply EqDec.eq_dec. Defined.
